lookup definition; replacing paths directory with paths-new

src/extensions/paths/Definitions.v
@@ -1,70 +1,130 @@
+(** printing |-#    %\vdash_{\#}%    #&vdash;<sub>&#35;</sub>#     *)
+(** printing |-##   %\vdash_{\#\#}%  #&vdash;<sub>&#35&#35</sub>#  *)
+(** printing |-##v  %\vdash_{\#\#v}% #&vdash;<sub>&#35&#35v</sub># *)
+(** printing |-!    %\vdash_!%       #&vdash;<sub>!</sub>#         *)
+(** remove printing ~ *)
+
+(** This proof uses the
+    #<a href="http://www.chargueraud.org/softs/tlc/">TLC</a>#
+    Coq library by Arthur Chargueraud. *)
+
 Set Implicit Arguments.
 
 Require Import LibLN.
-Require Import Coq.Program.Equality.
-
-(* ###################################################################### *)
-(* ###################################################################### *)
-(** * Definitions *)
-
-(* ###################################################################### *)
-(** ** Syntax *)
+Require Import String List.
 
 Parameter typ_label: Set.
 Parameter trm_label: Set.
 
+(** * Abstract Syntax *)
+
+(** *** Variables ([x], [y], [z])
+    The proof represents variables using the
+    #<a href="http://www.chargueraud.org/softs/ln/">locally nameless representation</a>#:
+    - [avar_b n] represents a variable using the de Bruijn index [n];
+    - [avar_f x] represents a free variable with name [x].
+    de Bruijn-indexed variables represent bound variables, whereas named variables represent free variables
+    that are in the evaluation context/type environment.  *)
+Inductive avar : Set :=
+  | avar_b : nat -> avar
+  | avar_f : var -> avar.
+
+(** *** Term and type members
+        Type member labels ([A], [B], [C]) and term (field) member labels ([a], [b], [c]).  *)
 Inductive label: Set :=
 | label_typ: typ_label -> label
 | label_trm: trm_label -> label.
 
-Inductive avar : Set :=
-  | avar_b : nat -> avar  (* bound var (de Bruijn index) *)
-  | avar_f : var -> avar. (* free var ("name"), refers to store or ctx *)
+(** The fields of a path in reverse order.
+    E.g. for a path x.a1.a2...an, a list [an, ..., a2, a1]. *)
+Definition fields := list trm_label.
 
-Inductive pathmode: Set := strong | gen.
+(** todo *)
+Inductive path :=
+  | p_sel : avar -> fields ->  path.
 
+(** *** Types
+    Types ([typ], [S], [T], [U]) and type declarations ([dec], [D]):
+    - [typ_top] represents [top];
+    - [typ_bot] represents [bottom];
+    - [typ_rcd d] represents a record type [d], where [d] is either a type or field declaration;
+    - [typ_and T U] represents an intersection type [T /\ U];
+    - [typ_sel x A] represents type selection [x.A];
+    - [typ_bnd T] represents a recursive type [mu(x: T)]; however, since [x] is bound in the recursive type,
+      it is referred to in [T] using the de Bruijn index 0, and is therefore omitted from the type representation;
+      we will denote recursive types as [mu(T)];
+    - [typ_all T U] represents the dependent function type [forall(x: T)U]; as in the previous case,
+      [x] represents a variable bound in [U], and is therefore omitted from the representation;
+      we will denote function types as [forall(T)U]. *)
 Inductive typ : Set :=
   | typ_top  : typ
   | typ_bot  : typ
-  | typ_rcd  : dec -> typ (* { D } *)
+  | typ_rcd  : dec -> typ
   | typ_and  : typ -> typ -> typ
-  | typ_path : path -> typ_label -> typ (* x.a1.a2. ... .an.L *)
-  | typ_bnd  : typ -> typ (* rec(x: T) *)
-  | typ_all  : typ -> typ -> typ (* all(x: S)T *)
-  | typ_sngl : path -> typ (* p.type *)
+  | typ_path : path -> typ_label -> typ
+  | typ_bnd  : typ -> typ
+  | typ_all  : typ -> typ -> typ
+(**
+  - [dec_typ A S T] represents a type declaraion [{A: S..T}];
+  - [dec_trm a T] represents a field declaration [{a: T}] . *)
 with dec : Set :=
-  | dec_typ  : typ_label -> typ -> typ -> dec (* A: S..U *)
-  | dec_trm  : trm_label -> pathmode -> typ -> dec (* {a: T} or {a:! T} *)
-with path : Set :=
-  | p_var : avar -> path
-  | p_sel : path -> trm_label -> path.
+  | dec_typ  : typ_label -> typ -> typ -> dec
+  | dec_trm  : trm_label -> typ -> dec.
 
-Notation "'{' a '[' m ']' T '}'" := (dec_trm a m T).
+(*Notation "'{' a ':' T '}'" := (dec_trm a T) (T at level 50).*)
 Notation "'{' A '>:' S '<:' T '}'" := (dec_typ A S T) (S at level 58).
 
+(** *** Terms
+  Terms ([trm], [t], [u]), values ([val], [v]),
+   member definitions ([def], [d] and [defs], [ds]):
+  - [trm_val v] represents a value [v];
+  - [trm_app p q] represents a function application [p q];
+  - [trm_let t u] represents a let binding [let x = t in u]; since x is bound in [u],
+    it is referred to in [u] using the de Bruijn index 0, and is therefore omitted from
+    the let-term representation; we will denote let terms as [let t in u];
+  - [trm_path p] represents a path [p]. *)
 Inductive trm : Set :=
   | trm_val  : val -> trm
-  | trm_app  : avar -> avar -> trm
-  | trm_let  : trm -> trm -> trm (* let x = t in u *)
+  | trm_app  : path -> path -> trm
+  | trm_let  : trm -> trm -> trm
   | trm_path : path -> trm
+(**
+  - [val_new T ds] represents the object [nu(x: T)ds]; the variable [x] is bound in [T]
+    and [ds] and is omitted from the representation;
+    we will denote new object definitions as [nu(T)ds];
+  - [val_lambda T t] represents a function [lambda(x: T)t]; again, [x] is bound in [t]
+    and is omitted;
+    we will denote lambda terms as [lambda(T)t. *)
 with val : Set :=
   | val_new  : typ -> defs -> val
   | val_lambda : typ -> trm -> val
+(**
+  - [def_typ A T] represents a type-member definition [{A = T}];
+  - [def_trm a t] represents a field definition [{a = t}]; *)
 with def : Set :=
   | def_typ  : typ_label -> typ -> def
   | def_trm  : trm_label -> trm -> def
+(**
+  [defs] represents a list of definitions that are part of an intersection
+  - [defs_nil] represents the empty list;
+  - [defs_cons d ds] represents a concatenation of the definition [d] to the definitions [ds]. *)
 with defs : Set :=
   | defs_nil : defs
   | defs_cons : defs -> def -> defs.
 
-(** *** Typing environment ("Gamma") *)
-Definition ctx := env typ.
+(** Shorthand definitions for variables and field selections *)
+Definition pavar (x: avar) := p_sel x nil.
+Definition pvar (x: var) := p_sel (avar_f x) nil.
+Definition tvar (x: var) := trm_path (pvar x).
+Definition sel_fields (p : path) (bs : list trm_label) :=
+  match p with
+  | p_sel x bs' => p_sel x (bs ++ bs')
+  end.
+Notation "p '•' a" := (sel_fields p (a :: nil)) (at level 5).
 
-(** *** Value environment ("store") *)
-Definition sto := env val.
+Hint Unfold pavar pvar tvar.
 
-(* ###################################################################### *)
-(** ** Definition list membership *)
+(** Helper functions to retrieve labels of declarations and definitions *)
 
 Definition label_of_def(d: def): label := match d with
 | def_typ L _ => label_typ L
@@ -73,7 +133,7 @@ end.
 
 Definition label_of_dec(D: dec): label := match D with
 | dec_typ L _ _ => label_typ L
-| dec_trm a _ _ => label_trm a
+| dec_trm m _   => label_trm m
 end.
 
 Fixpoint get_def(l: label)(ds: defs): option def :=
@@ -83,34 +143,37 @@ match ds with
 end.
 
 Definition defs_has(ds: defs)(d: def) := get_def (label_of_def d) ds = Some d.
+
 Definition defs_hasnt(ds: defs)(l: label) := get_def l ds = None.
 
-Inductive record_has: typ -> dec -> Prop :=
-| rh_one : forall D,
-    record_has (typ_rcd D) D
-| rh_andl : forall T U D,
-    record_has T D ->
-    record_has (typ_and T U) D
-| rh_andr : forall T U D,
-    record_has U D ->
-    record_has (typ_and T U) D.
+(** Typing environment ([G]) *)
+Definition ctx := env typ.
 
-(* ###################################################################### *)
-(** ** Opening *)
+(** A list of field paths, representing a list of paths
+    that start with the same variable. *)
+Definition paths := list fields.
 
-(** Variable opening replaces in some syntax a bound variable with dangling index (k)
-   by a free variable x. *)
+(** The sequence of variable-to-value let bindings, [(let x = v in)*],
+     is represented as a value environment that maps variables to values: *)
+Definition sta := env val.
+
+(** * Opening *)
+(** Opening takes a bound variable that is represented with a de Bruijn index [k]
+    and replaces it by a named variable or path [u].
+    The following functions define opening on paths, types, declarations, terms,
+    values, and definitions.
+
+    We will denote an identifier [X] opened with a variable [y] as [X^y]. *)
 
 Definition open_rec_avar (k: nat) (u: var) (a: avar) : avar :=
   match a with
   | avar_b i => If k = i then avar_f u else avar_b i
   | avar_f x => avar_f x
-  end.
+end.
 
-Fixpoint open_rec_path (k: nat) (u: var) (p: path): path :=
+Definition open_rec_path (k: nat) (u: var) (p: path): path :=
   match p with
-  | p_var x   => p_var (open_rec_avar k u x)
-  | p_sel q m => p_sel (open_rec_path k u q) m
+  | p_sel x bs => p_sel (open_rec_avar k u x) bs
   end.
 
 Fixpoint open_rec_typ (k: nat) (u: var) (T: typ): typ :=
@@ -122,19 +185,18 @@ Fixpoint open_rec_typ (k: nat) (u: var) (T: typ): typ :=
   | typ_path p L   => typ_path (open_rec_path k u p) L
   | typ_bnd T      => typ_bnd (open_rec_typ (S k) u T)
   | typ_all T1 T2  => typ_all (open_rec_typ k u T1) (open_rec_typ (S k) u T2)
-  | typ_sngl p     => typ_sngl (open_rec_path k u p)
   end
 with open_rec_dec (k: nat) (u: var) (D: dec): dec :=
   match D with
   | { L >: T <: U } => { L >: open_rec_typ k u T <: open_rec_typ k u U }
-  | { a [m] T } => { a [m] open_rec_typ k u T }
+  | dec_trm a T => dec_trm a (open_rec_typ k u T)
   end.
 
 Fixpoint open_rec_trm (k: nat) (u: var) (t: trm): trm :=
   match t with
   | trm_val v      => trm_val (open_rec_val k u v)
   | trm_path p     => trm_path (open_rec_path k u p)
-  | trm_app f a    => trm_app (open_rec_avar k u f) (open_rec_avar k u a)
+  | trm_app p q    => trm_app (open_rec_path k u p) (open_rec_path k u q)
   | trm_let t1 t2  => trm_let (open_rec_trm k u t1) (open_rec_trm (S k) u t2)
   end
 with open_rec_val (k: nat) (u: var) (v: val): val :=
@@ -162,23 +224,26 @@ Definition open_def  u d := open_rec_def   0 u d.
 Definition open_defs u l := open_rec_defs  0 u l.
 Definition open_path u p := open_rec_path  0 u p.
 
-Notation "t '|^' x" := (open_trm x t) (at level 35).
-Notation "T '||^' x" := (open_typ x T) (at level 35).
-Notation "ds '|||^' x" := (open_defs x ds) (at level 35).
+Definition open_paths u ps := map (open_path u) ps.
 
-(** Path oopening replaces in some syntax a bound variable with dangling index (k)
-   by a path p. *)
+(** Path opening replaces in some syntax a bound variable with dangling index (k)
+    by a path p. *)
 
 Definition open_rec_avar_p (k: nat) (u: path) (a: avar) : path :=
   match a with
-  | avar_b i => If k = i then u else p_var (avar_b i)
-  | avar_f x => p_var (avar_f x)
+  | avar_b i => If k = i then u else pavar (avar_b i)
+  | avar_f x => pvar x
   end.
 
-Fixpoint open_rec_path_p (k: nat) (u: path) (p: path): path :=
-  match p with
-  | p_var x   => open_rec_avar_p k u x
-  | p_sel q m => p_sel (open_rec_path_p k u q) m
+(* example:            (0.a.b    ^ y.c.d    == y.c.d.a.b
+   our representation: (0 [b, a] ^ y [d, c] == y [b, a, d, c] *)
+Definition open_rec_path_p (k: nat) (u: path) (p: path): path :=
+  match p, u with
+  | p_sel x bs, p_sel y cs=>
+    match x with
+    | avar_b i => If k = i then p_sel y (bs ++ cs) else p (* maintaining reverse order of fields *)
+    | avar_f x => p
+    end
   end.
 
 Fixpoint open_rec_typ_p (k: nat) (u: path) (T: typ): typ :=
@@ -190,35 +255,62 @@ Fixpoint open_rec_typ_p (k: nat) (u: path) (T: typ): typ :=
   | typ_path p L   => typ_path (open_rec_path_p k u p) L
   | typ_bnd T      => typ_bnd (open_rec_typ_p (S k) u T)
   | typ_all T1 T2  => typ_all (open_rec_typ_p k u T1) (open_rec_typ_p (S k) u T2)
-  | typ_sngl p     => typ_sngl (open_rec_path_p k u p)
   end
 with open_rec_dec_p (k: nat) (u: path) (D: dec): dec :=
   match D with
   | { L >: T <: U } => { L >: open_rec_typ_p k u T <: open_rec_typ_p k u U }
-  | { a [m] T} => { a [m] open_rec_typ_p k u T }
+  | dec_trm a T => dec_trm a (open_rec_typ_p k u T)
+  end.
+
+Fixpoint open_rec_trm_p (k: nat) (u: path) (t: trm): trm :=
+  match t with
+  | trm_val v      => trm_val (open_rec_val_p k u v)
+  | trm_path p     => trm_path (open_rec_path_p k u p)
+  | trm_app p q    => trm_app (open_rec_path_p k u p) (open_rec_path_p k u q)
+  | trm_let t1 t2  => trm_let (open_rec_trm_p k u t1) (open_rec_trm_p (S k) u t2)
+  end
+with open_rec_val_p (k: nat) (u: path) (v: val): val :=
+  match v with
+  | val_new T ds => val_new (open_rec_typ_p (S k) u T) (open_rec_defs_p (S k) u ds)
+  | val_lambda T e => val_lambda (open_rec_typ_p k u T) (open_rec_trm_p (S k) u e)
+  end
+with open_rec_def_p (k: nat) (u: path) (d: def): def :=
+  match d with
+  | def_typ L T => def_typ L (open_rec_typ_p k u T)
+  | def_trm m e => def_trm m (open_rec_trm_p k u e)
+  end
+with open_rec_defs_p (k: nat) (u: path) (ds: defs): defs :=
+  match ds with
+  | defs_nil => defs_nil
+  | defs_cons tl d => defs_cons (open_rec_defs_p k u tl) (open_rec_def_p k u d)
   end.
 
 Definition open_avar_p u a := open_rec_avar_p  0 u a.
 Definition open_typ_p  u t := open_rec_typ_p   0 u t.
 Definition open_dec_p  u D := open_rec_dec_p   0 u D.
 Definition open_path_p u p := open_rec_path_p  0 u p.
+Definition open_trm_p  u t := open_rec_trm_p   0 u t.
+Definition open_val_p  u v := open_rec_val_p   0 u v.
+Definition open_def_p  u d := open_rec_def_p   0 u d.
+Definition open_defs_p u l := open_rec_defs_p 0 u l.
 
+(** * Free variables
+      Functions that retrieve the free variables of a symbol. *)
 
-(* ###################################################################### *)
-(** ** Free variables *)
-
+(** Free variable in a variable. *)
 Definition fv_avar (a: avar) : vars :=
   match a with
   | avar_b i => \{}
   | avar_f x => \{x}
   end.
 
+(** Free variable in a path. *)
 Fixpoint fv_path (p: path) : vars :=
   match p with
-  | p_var x   => fv_avar x
-  | p_sel q L => fv_path q
+  | p_sel x bs => fv_avar x
   end.
 
+(** Free variables in a type or declaration. *)
 Fixpoint fv_typ (T: typ) : vars :=
   match T with
   | typ_top        => \{}
@@ -228,19 +320,19 @@ Fixpoint fv_typ (T: typ) : vars :=
   | typ_path p L   => fv_path p
   | typ_bnd T      => fv_typ T
   | typ_all T1 T2  => (fv_typ T1) \u (fv_typ T2)
-  | typ_sngl p     => fv_path p
   end
 with fv_dec (D: dec) : vars :=
   match D with
   | { L >: T <: U } => (fv_typ T) \u (fv_typ U)
-  | { a [m] T } => fv_typ T
+  | dec_trm a T => fv_typ T
   end.
 
+(** Free variables in a term, value, or definition. *)
 Fixpoint fv_trm (t: trm) : vars :=
   match t with
   | trm_val v        => (fv_val v)
   | trm_path p       => (fv_path p)
-  | trm_app f a      => (fv_avar f) \u (fv_avar a)
+  | trm_app p q      => (fv_path p) \u (fv_path q)
   | trm_let t1 t2    => (fv_trm t1) \u (fv_trm t2)
   end
 with fv_val (v: val) : vars :=
@@ -259,13 +351,26 @@ with fv_defs(ds: defs) : vars :=
   | defs_cons tl d   => (fv_defs tl) \u (fv_def d)
   end.
 
+(** Free variables in the range (types) of a context *)
 Definition fv_ctx_types(G: ctx): vars := (fv_in_values (fun T => fv_typ T) G).
+Definition fv_sta_vals(s: sta): vars := (fv_in_values (fun v => fv_val v) s).
 
+(** ** Record types *)
+(** In the proof, it is useful to be able to distinguish record types from
+    other types. A record type is a concatenation of type declarations with equal
+    bounds [{A: T..T}] and field declarations [{a: T}]. *)
+
+(** A record declaration is either a type declaration with equal bounds,
+    or a field declaration.*)
 Inductive record_dec : dec -> Prop :=
-| rd_typ : forall A T, record_dec { A >: T <: T }
-| rd_trm : forall a m T, record_dec { a [m] T }.
+| rd_typ : forall A T, record_dec (dec_typ A T T)
+| rd_trm : forall a T, inert_typ T -> record_dec (dec_trm a T)
 
-Inductive record_typ : typ -> fset label -> Prop :=
+(** Given a record declaration, a [record_typ] keeps track of the declaration's
+    field member labels (i.e. names of fields) and type member labels
+    (i.e. names of abstract type members). [record_typ] also requires that the
+    labels are distinct.  *)
+with record_typ : typ -> fset label -> Prop :=
 | rt_one : forall D l,
   record_dec D ->
   l = label_of_dec D ->
@@ -275,574 +380,432 @@ Inductive record_typ : typ -> fset label -> Prop :=
   record_dec D ->
   l = label_of_dec D ->
   l \notin ls ->
-  record_typ (typ_and T (typ_rcd D)) (union ls \{l}).
+  record_typ (typ_and T (typ_rcd D)) (union ls \{l})
 
+(** ** Inert types
+       A type is inert if it is either a dependent function type, or a recursive type
+       whose type declarations have equal bounds (enforced through [record_type]). #<br>#
+       For example, the following types are inert:
+       - [lambda(x: S)T]
+       - [mu(x: {a: T} /\ {B: U..U})]
+       - [mu(x: {C: {A: T..U}..{A: T..U}})]
+       And the following types are not inert:
+       - [{a: T}]
+       - [{B: U..U}]
+       - [top]
+       - [x.A]
+       - [mu(x: {B: S..T})], where [S <> T]. *)
+with inert_typ : typ -> Prop :=
+  | inert_typ_all : forall S T, inert_typ (typ_all S T)
+  | inert_typ_bnd : forall T ls,
+      record_typ T ls ->
+      inert_typ (typ_bnd T).
+
+(** Given a type [T = D1 /\ D2 /\ ... /\ Dn] and member declaration [D], [record_has T D] tells whether
+    [D] is contained in the intersection of [Di]'s. *)
+Inductive record_has: typ -> dec -> Prop :=
+| rh_one : forall D,
+    record_has (typ_rcd D) D
+| rh_andl : forall T U D,
+    record_has T D ->
+    record_has (typ_and T U) D
+| rh_andr : forall T U D,
+    record_has U D ->
+    record_has (typ_and T U) D.
+
+(** A [record_type] is a [record_typ] with an unspecified set of labels. The meaning
+    of [record_type] is an intersection of type/field declarations with distinct labels. *)
 Definition record_type T := exists ls, record_typ T ls.
 
-(* Definition (Inert types)
-
-A type is inert if it of the form
-  all(x: S)T
-  rec(x: T), where T is a record type
- *)
-
-Inductive inert_typ : typ -> Prop :=
-  | inert_typ_all : forall S T, inert_typ (typ_all S T) (* all(x: S)T *)
-  | inert_typ_bnd : forall T,
-      (* a record type is ands of record decs *)
-      record_type T ->
-      inert_typ (typ_bnd T). (* rec(x:T) *)
-
-(* Definition (Inert context)
-
-A context is inert if it is of the form
-  {}
-  G, x : T where G is a inert context and T is a inert type *)
-
+(** An inert context is a typing context whose range consists only of inert types. *)
 Inductive inert : ctx -> Prop :=
   | inert_empty : inert empty
-  | inert_all : forall pre x T,
-      inert pre ->
+  | inert_all : forall G x T,
+      inert G ->
       inert_typ T ->
-      x # pre ->
-      inert (pre & x ~ T).
+      x # G ->
+      inert (G & x ~ T).
 
-(* ###################################################################### *)
-(** ** Operational Semantics *)
+(** * Typing Rules *)
 
-Reserved Notation "t1 '/' st1 '⇒' t2 '/' st2" (at level 40, t2 at level 39).
+Reserved Notation "G '⊢' t ':' T" (at level 40, t at level 59).
+Reserved Notation "G '⊢' T '<:' U" (at level 40, T at level 59).
+Reserved Notation "x ';' bs ';' P ';' G '⊢' d ':' D"
+         (at level 40, bs at level 39, P at level 39, G at level 39, d at level 59).
+Reserved Notation "x ';' bs ';' P ';' G '⊢' ds '::' D"
+         (at level 40, bs at level 39, P at level 39, G at level 39, ds at level 59).
+(* Reserved Notation "P '⊢' p '<' q" (at level 40, p at level 59). *)
 
-Inductive red : trm -> sto -> trm -> sto -> Prop :=
-| red_sel : forall x a s t T ds,
-    binds x (val_new T ds) s ->
-    defs_has (ds |||^ x) (def_trm a t) ->
-    trm_path (p_sel (p_var (avar_f x)) a) / s ⇒ t / s
-| red_path : forall p a b s,
-    trm_path (p_sel (p_sel p a) b) / s ⇒
-             trm_let (trm_path (p_sel p a)) (trm_path (p_sel (p_var (avar_b 0)) b)) / s
-| red_app : forall x y s T t,
-    binds x (val_lambda T t) s ->
-    trm_app (avar_f x) (avar_f y) / s ⇒ t |^ y / s
-| red_let : forall v t s x,
-    x # s ->
-    trm_let (trm_val v) t / s ⇒ t |^ x / s & x ~ v
-| red_let_var : forall t s x,
-    trm_let (trm_path (p_var (avar_f x))) t / s ⇒ t |^ x / s
-| red_let_tgt : forall t u s t' s',
-    t / s ⇒ t' / s' ->
-    trm_let t u / s ⇒ trm_let t' u / s'
-where "t1 '/' st1 '⇒' t2 '/' st2" := (red t1 st1 t2 st2).
+Definition uniq := LibList.No_duplicates.
 
-(* ###################################################################### *)
-(** ** Typing *)
+Inductive path_precedes : paths -> fields -> fields -> Prop :=
+| pp: forall P P1 P2 p q,
+    P = app P1 P2 ->
+    uniq P ->
+    In p P1 ->
+    In q P2 ->
+    path_precedes P p q.
 
-(* is a type inert or a singleton type? *)
-Inductive inert_sngl: typ -> Prop :=
-| is_inert: forall T, inert_typ T -> inert_sngl T
-| is_sngl: forall p, inert_sngl (typ_sngl p).
-
-Reserved Notation "G '|-' t ':' T" (at level 40, t at level 59).
-Reserved Notation "G '|-' T '<:' U" (at level 40, T at level 59).
-Reserved Notation "G '|-\||/' p ':' T" (at level 40, p at level 59).
-Reserved Notation "G '&&' z '~' T '|-' d ':' D" (at level 39, z at level 26, T at level 39, d at level 59).
-Reserved Notation "G '&&' z '~' T '|-' ds '::' U" (at level 39, z at level 26, T at level 39, ds at level 59).
-
+(** ** Term typing [G ⊢ t: T] *)
 Inductive ty_trm : ctx -> trm -> typ -> Prop :=
-| ty_var : forall G x T,
+
+(** [G(x) = T]   #<br>#
+    [ok G]       #<br>#
+    [――――――――]   #<br>#
+    [G ⊢ x: T]  *)
+| ty_var : forall x T G,
     binds x T G ->
-    G |- trm_path (p_var (avar_f x)) : T
+    ok G ->
+    G ⊢ tvar x : T
+
+(** [G, z: T ⊢ t^z: U^z]     #<br>#
+    [z fresh]                #<br>#
+    [――――――――――――――――――――――] #<br>#
+    [G ⊢ lambda(T)t: forall(T)U]      *)
 | ty_all_intro : forall L G T t U,
-    (forall x, x \notin L ->
-      G & x ~ T |- t |^ x : U ||^ x) ->
-    G |- trm_val (val_lambda T t) : typ_all T U
-| ty_all_elim : forall G x y S T,
-    G |- trm_path (p_var (avar_f x)) : typ_all S T ->
-    G |- trm_path (p_var (avar_f y)) : S ->
-    G |- trm_app (avar_f x) (avar_f y) : T ||^ y
-| ty_new_intro : forall L G T ds,
-    (forall x, x \notin L ->
-      G && x ~ T ||^ x |- ds |||^ x :: T ||^ x) ->
-    G |- trm_val (val_new T ds) : typ_bnd T
-| ty_fld_elim : forall G p a T,
-    G |- trm_path p : typ_rcd { a [gen] T } ->
-    G |- trm_path (p_sel p a) : T
+    (forall z, z \notin L ->
+      G & z ~ T ⊢ open_trm z t : open_typ z U) ->
+    G ⊢ trm_val (val_lambda T t) : typ_all T U
+
+(** [G ⊢ p: forall(S)T] #<br>#
+    [G ⊢ q: S]     #<br>#
+    [――――――――――――] #<br>#
+    [G ⊢ p q: T^q]     *)
+| ty_all_elim : forall G p q S T,
+    G ⊢ trm_path p : typ_all S T ->
+    G ⊢ trm_path q : S ->
+    G ⊢ trm_app p q : open_typ_p p T
+
+(** [z; P; G, z: T^z ⊢ ds^z :: T^z]    #<br>#
+    [z fresh]                          #<br>#
+    [―――――――――――――――――――――――――――――――]  #<br>#
+    [G ⊢ nu(T)ds :: mu(T)]             *)
+| ty_new_intro : forall L G T ds P,
+    (forall z, z \notin L ->
+      z; nil; P; G & (z ~ open_typ z T) ⊢ open_defs z ds :: open_typ z T) ->
+    G ⊢ trm_val (val_new T ds) : typ_bnd T
+
+(** [G ⊢ p: {a: T}] #<br>#
+    [―――――――――――――] #<br>#
+    [G ⊢ p.a: T]        *)
+| ty_new_elim : forall G p a T,
+    G ⊢ trm_path p : typ_rcd (dec_trm a T) ->
+    G ⊢ trm_path p•a : T
+
+(** [G ⊢ t: T]          #<br>#
+    [G, x: T ⊢ u^x: U]  #<br>#
+    [x fresh]           #<br>#
+    [―――――――――――――――――] #<br>#
+    [G ⊢ let t in u: U]     *)
 | ty_let : forall L G t u T U,
-    G |- t : T ->
+    G ⊢ t : T ->
     (forall x, x \notin L ->
-      G & x ~ T |- u |^ x : U) ->
-    G |- trm_let t u : U
-| ty_rec_intro : forall G x T,
-    G |- trm_path (p_var (avar_f x)) : T ||^ x ->
-    G |- trm_path (p_var (avar_f x)) : typ_bnd T
-| ty_rec_elim : forall G x T,
-    G |- trm_path (p_var (avar_f x)) : typ_bnd T ->
-    G |- trm_path (p_var (avar_f x)) : open_typ x T
-| ty_and_intro : forall G x T U,
-    G |- trm_path (p_var (avar_f x)) : T ->
-    G |- trm_path (p_var (avar_f x)) : U ->
-    G |- trm_path (p_var (avar_f x)) : typ_and T U
-| ty_sngl_intro : forall G x T,
-    G |- trm_path (p_var (avar_f x)): T ->
-    G |- trm_path (p_var (avar_f x)) : typ_sngl (p_var (avar_f x))
+      G & x ~ T ⊢ open_trm x u : U) ->
+    G ⊢ trm_let t u : U
+
+(** [G ⊢ p: T^p]   #<br>#
+    [――――――――――――] #<br>#
+    [G ⊢ p: mu(T)]     *)
+| ty_rec_intro : forall G p T,
+    G ⊢ trm_path p : open_typ_p p T ->
+    G ⊢ trm_path p : typ_bnd T
+
+(** [G ⊢ p: mu(T)] #<br>#
+    [――――――――――――] #<br>#
+    [G ⊢ p: T^p]   *)
+| ty_rec_elim : forall G p T,
+    G ⊢ trm_path p : typ_bnd T ->
+    G ⊢ trm_path p : open_typ_p p T
+
+(** [G ⊢ p: T]     #<br>#
+    [G ⊢ p: U]     #<br>#
+    [――――――――――――] #<br>#
+    [G ⊢ p: T /\ U]     *)
+| ty_and_intro : forall G p T U,
+    G ⊢ trm_path p : T ->
+    G ⊢ trm_path p : U ->
+    G ⊢ trm_path p : typ_and T U
+
+(** [G ⊢ t: T]   #<br>#
+    [G ⊢ T <: U] #<br>#
+    [――――――――――] #<br>#
+    [G ⊢ t: U]   *)
 | ty_sub : forall G t T U,
-    G |- t : T ->
-    G |- T <: U ->
-    G |- t : U
-where "G '|-' t ':' T" := (ty_trm G t T)
+    G ⊢ t : T ->
+    G ⊢ T <: U ->
+    G ⊢ t : U
+where "G '⊢' t ':' T" := (ty_trm G t T)
 
-with ty_path : ctx -> path -> typ -> Prop :=
-| ty_p_intro: forall G x T,
-    G |- trm_path (p_var (avar_f x)): T ->
-    G |-\||/ p_var (avar_f x): T
-| ty_p_rec_elim : forall G p T,
-    G |-\||/ p : typ_bnd T ->
-    G |-\||/ p : open_typ_p p T
-| ty_p_and_elim1 : forall G p T U,
-    G |-\||/ p: typ_and T U ->
-    G |-\||/ p: T
-| ty_p_and_elim_2 : forall G p T U,
-    G |-\||/ p: typ_and T U ->
-    G |-\||/ p: U
-| ty_p_fld_elim : forall G p a T,
-    G |-\||/ p: typ_rcd {a [strong] T} ->
-    inert_sngl T ->
-    G |-\||/ p_sel p a : T
-| ty_p_sub : forall G p T U,
-    G |-\||/ p: T ->
-    G |- T <: U ->
-    G |-\||/ p: U
-where "G '|-\||/' p ':' T" := (ty_path G p T)
+(** ** Single-definition typing [x; bs; P; G ⊢ d: D] *)
+with ty_def : var -> fields -> paths -> ctx -> def -> dec -> Prop :=
+(** [x; bs; G ⊢ {A = T}: {A: T..T}]   *)
+| ty_def_typ : forall x bs P G A T,
+    x; bs; P; G ⊢ def_typ A T : dec_typ A T T
 
-with ty_def : ctx -> var -> typ -> def -> dec -> Prop := (* Γ; z: U |- d: T U *)
-| ty_def_typ : forall z G A T U,
-    G && z ~ U |- def_typ A T : { A >: T <: T }
-| ty_def_trm : forall z G a t T U,
-    G & z ~ U |- t : T ->
-    G && z ~ U |- def_trm a t : { a [gen] T }
-| ty_def_path : forall z G a p U T,
-    G |-\||/ p : T ->
-    G && z ~ U |- def_trm a (trm_path p) : { a [strong] T }
-| ty_def_val : forall G z U v T a,
-    G & z ~ U |- trm_val v : T ->
-    G && z ~ U |- def_trm a (trm_val v) : { a [strong] T }
-where "G '&&' z '~' T '|-' d ':' D" := (ty_def G z T d D)
+(** [G ⊢ lambda(T)t: U]                     #<br>#
+    [―――――――――――――――――――――――――――――――――――――] #<br>#
+    [x; bs; P; G ⊢ {b = lambda(T)t: U}: {b: T}] *)
+ | ty_def_all : forall x bs P G T t b U,
+    G ⊢ trm_val (val_lambda T t) : U ->
+    inert_typ U ->
+    x; bs; P; G ⊢ def_trm b (trm_val (val_lambda T t)) : dec_trm b U
 
-with ty_defs : ctx -> var -> typ -> defs -> typ -> Prop :=
-| ty_defs_one : forall z G d D U,
-    G && z ~ U |- d : D ->
-    G && z ~ U |- defs_cons defs_nil d :: typ_rcd D
-| ty_defs_cons : forall G ds d z T U D,
-    G && z ~ U |- ds :: T ->
-    G && z ~ U |- d : D ->
+(** [x; (b, bs); P; G ⊢ ds^p.b: T^p.b]             #<br>#
+    [―――――――――――――――――――――――――――――――――――――] #<br>#
+    [x; bs; P; G ⊢ {b = nu(T)ds}: {b: T}]    *)
+ | ty_def_new : forall x bs b P G ds T p,
+     p = p_sel (avar_f x) bs ->
+     inert_typ (typ_bnd T) ->
+     x; (b :: bs); P; G ⊢ open_defs_p p•b ds :: open_typ_p p•b T ->
+     x; bs; P; G ⊢ def_trm b (trm_val (val_new T ds)) : dec_trm b (typ_bnd T)
+
+(** if [x == head(q)] then [P ⊢ (b, bs) < fields(q)] #<br>#
+    [G ⊢ q: T]                                       #<br>#
+    [――――――――――――――――――――――――――――――――――――――――――――――] #<br>#
+    [x; bs; P; G ⊢ {a = q}: {a: T}]                  *)
+ | ty_def_path : forall x bs P G q y cs b T,
+    G ⊢ trm_path q: T ->
+    inert_typ T ->
+    q = p_sel (avar_f y) cs ->
+    (x = y -> path_precedes P (b :: bs) cs) ->
+    x; bs; P; G ⊢ def_trm b (trm_path q) : dec_trm b T
+
+where "x ';' bs ';' P ';' G '⊢' d ':' D" := (ty_def x bs P G d D)
+
+(** ** Multiple-definition typing [x; bs; P; G ⊢ ds :: T] *)
+with ty_defs : var -> fields -> paths -> ctx -> defs -> typ -> Prop :=
+(** [x; bs; P G ⊢ d: D]                #<br>#
+    [――――――――――――――――――――――――――――――――] #<br>#
+    [x; bs; P; G ⊢ d ++ defs_nil : D]   *)
+| ty_defs_one : forall x bs P G d D,
+    x; bs; P; G ⊢ d : D ->
+    x; bs; P; G ⊢ defs_cons defs_nil d :: typ_rcd D
+
+(** [x; bs; G ⊢ ds :: T]           #<br>#
+    [x; bs; G ⊢ d: D]              #<br>#
+    [d \notin ds]                  #<br>#
+    [―――――――――――――――――――――――――――]  #<br>#
+    [x; bs; G ⊢ ds ++ d : T /\ D]   *)
+| ty_defs_cons : forall x bs P G d ds D T,
+    x; bs; P; G ⊢ ds :: T ->
+    x; bs; P; G ⊢ d : D ->
     defs_hasnt ds (label_of_def d) ->
-    G && z ~ U |- defs_cons ds d :: typ_and T (typ_rcd D)
-where "G '&&' z '~' T '|-' ds '::' U" := (ty_defs G z T ds U)
+    x; bs; P; G ⊢ defs_cons ds d :: typ_and T (typ_rcd D)
+where "x ';' bs ';' P ';' G '⊢' ds '::' T" := (ty_defs x bs P G ds T)
 
+(** ** Subtyping [ G ⊢ T <: U] *)
 with subtyp : ctx -> typ -> typ -> Prop :=
+
+(** [G ⊢ T <: top] *)
 | subtyp_top: forall G T,
-    G |- T <: typ_top
+    G ⊢ T <: typ_top
+
+(** [G ⊢ bot <: T] *)
 | subtyp_bot: forall G T,
-    G |- typ_bot <: T
+    G ⊢ typ_bot <: T
+
+(** [G ⊢ T <: T] *)
 | subtyp_refl: forall G T,
-    G |- T <: T
+    G ⊢ T <: T
+
+(** [G ⊢ S <: T]     #<br>#
+    [G ⊢ T <: U]     #<br>#
+    [――――――――――]     #<br>#
+    [G ⊢ S <: U]         *)
 | subtyp_trans: forall G S T U,
-    G |- S <: T ->
-    G |- T <: U ->
-    G |- S <: U
+    G ⊢ S <: T ->
+    G ⊢ T <: U ->
+    G ⊢ S <: U
+
+(** [G ⊢ T /\ U <: T] *)
 | subtyp_and11: forall G T U,
-    G |- typ_and T U <: T
+    G ⊢ typ_and T U <: T
+
+(** [G ⊢ T /\ U <: U] *)
 | subtyp_and12: forall G T U,
-    G |- typ_and T U <: U
+    G ⊢ typ_and T U <: U
+
+(** [G ⊢ S <: T]       #<br>#
+    [G ⊢ S <: U]       #<br>#
+    [――――――――――――――]   #<br>#
+    [G ⊢ S <: T /\ U]          *)
 | subtyp_and2: forall G S T U,
-    G |- S <: T ->
-    G |- S <: U ->
-    G |- S <: typ_and T U
-| subtyp_fld: forall G a T U,
-    G |- T <: U ->
-    G |- typ_rcd { a [gen] T } <: typ_rcd { a [gen] U }
-| subtyp_typ: forall G A S1 T1 S2 T2,
-    G |- S2 <: S1 ->
-    G |- T1 <: T2 ->
-    G |- typ_rcd { A >: S1 <: T1 } <: typ_rcd { A >: S2 <: T2 }
+    G ⊢ S <: T ->
+    G ⊢ S <: U ->
+    G ⊢ S <: typ_and T U
+
+(** [G ⊢ T <: U]           #<br>#
+    [――――――――――――――――――――] #<br>#
+    [G ⊢ {a: T} <: {a: U}] *)
+| subtyp_fld: forall G T U a,
+    G ⊢ T <: U ->
+    G ⊢ typ_rcd (dec_trm a T) <: typ_rcd (dec_trm a U)
+
+(** [G ⊢ S2 <: S1]                   #<br>#
+    [G ⊢ T1 <: T2]                   #<br>#
+    [――――――――――――――――――――――――――――――] #<br>#
+    [G ⊢ {A: S1..T1} <: {A: S2..T2}]     *)
+| subtyp_typ: forall G S1 S2 T1 T2 A,
+    G ⊢ S2 <: S1 ->
+    G ⊢ T1 <: T2 ->
+    G ⊢ typ_rcd (dec_typ A S1 T1) <: typ_rcd (dec_typ A S2 T2)
+
+(** [G ⊢ x: {A: S..T}] #<br>#
+    [――――――――――――――――] #<br>#
+    [G ⊢ S <: x.A]     *)
 | subtyp_sel2: forall G p A S T,
-    G |-\||/ p : typ_rcd { A >: S <: T } ->
-    G |- S <: typ_path p A
+    G ⊢ trm_path p : typ_rcd (dec_typ A S T) ->
+    G ⊢ S <: typ_path p A
+
+(** [G ⊢ x: {A: S..T}] #<br>#
+    [――――――――――――――――] #<br>#
+    [G ⊢ x.A <: T]     *)
 | subtyp_sel1: forall G p A S T,
-    G |-\||/ p : typ_rcd { A >: S <: T } ->
-    G |- typ_path p A <: T
-| subtyp_sngl_sel1: forall G p q A S U,
-    G |-\||/ p: typ_sngl q ->
-    G |- trm_path q: typ_rcd { A >: S <: U } ->
-    G |- typ_path p A <: typ_path q A
-| subtyp_sngl_sel2: forall G p q A S U,
-    G |-\||/ p: typ_sngl q ->
-    G |- trm_path q: typ_rcd { A >: S <: U } ->
-    G |- typ_path q A <: typ_path p A
-| subtyp_all: forall L G S1 T1 S2 T2,
-    G |- S2 <: S1 ->
-    (forall x, x \notin L ->
-       G & x ~ S2 |- T1 ||^ x <: T2 ||^ x) ->
-    G |- typ_all S1 T1 <: typ_all S2 T2
-| subtyp_path: forall G a T,
-    G |- typ_rcd { a [strong] T } <: typ_rcd { a [gen] T }
-where "G '|-' T '<:' U" := (subtyp G T U).
+    G ⊢ trm_path p : typ_rcd (dec_typ A S T) ->
+    G ⊢ typ_path p A <: T
 
-Reserved Notation "G '|-!' t ':' T" (at level 40, t at level 59).
+(** [G ⊢ S2 <: S1]                #<br>#
+    [G, x: S2 ⊢ T1^x <: T2^x]     #<br>#
+    [x fresh]                     #<br>#
+    [―――――――――――――――――――――――]     #<br>#
+    [G ⊢ forall(S1)T1 <: forall(S2)T2]      *)
+| subtyp_all : forall (L : fset var) (G : ctx) (S1 T1 S2 T2 : typ),
+    G ⊢ S2 <: S1 ->
+    (forall x : var, x \notin L -> G & x ~ S2 ⊢ open_typ x T1 <: open_typ x T2) ->
+      G ⊢ typ_all S1 T1 <: typ_all S2 T2
+where "G '⊢' T '<:' U" := (subtyp G T U).
 
-Inductive ty_trm_p : ctx -> trm -> typ -> Prop :=
-| ty_var_p : forall G x T,
-    binds x T G ->
-    G |-! trm_path (p_var (avar_f x)) : T
-| ty_all_intro_p : forall L G T t U,
-    (forall x, x \notin L ->
-      G & x ~ T |- t |^ x : U ||^ x) ->
-    G |-! trm_val (val_lambda T t) : typ_all T U
-| ty_new_intro_p : forall L G T ds,
-    (forall x, x \notin L ->
-      G && x ~ T ||^ x |- ds |||^ x :: T ||^ x) ->
-    G |-! trm_val (val_new T ds) : typ_bnd T
-| ty_rec_elim_p : forall G p T,
-    G |-! trm_path p : typ_bnd T ->
-    G |-! trm_path p : open_typ_p p T
-| ty_and1_p : forall G p T U,
-    G |-! trm_path p : typ_and T U ->
-    G |-! trm_path p : T
-| ty_and2_p : forall G p T U,
-    G |-! trm_path p : typ_and T U ->
-    G |-! trm_path p : U
-| ty_fld_elim_p : forall G p a T,
-    G |-! trm_path p: typ_rcd {a [strong] T} ->
-    inert_sngl T ->
-    G |-! trm_path (p_sel p a): T
-where "G '|-!' t ':' T" := (ty_trm_p G t T).
+(** * Well-typed stacks *)
 
-Reserved Notation "G '|-#' t ':' T" (at level 40, t at level 59).
-Reserved Notation "G '|-#' T '<:' U" (at level 40, T at level 59).
-Reserved Notation "G '|-#\||/' p ':' T" (at level 40, p at level 59).
+(** The operational semantics is defined in terms of pairs [(s, t)], where
+    [s] is a stack and [t] is a term.
+    Given a typing [G ⊢ (s, t): T], [well_typed] establishes a correspondence
+    between [G] and the stack [s].
 
-Inductive ty_trm_t : ctx -> trm -> typ -> Prop :=
-| ty_var_t : forall G x T,
-    binds x T G ->
-    G |-# trm_path (p_var (avar_f x)) : T
-| ty_all_intro_t : forall L G T t U,
-    (forall x, x \notin L ->
-      G & x ~ T |- t |^ x : U ||^ x) ->
-    G |-# trm_val (val_lambda T t) : typ_all T U
-| ty_all_elim_t : forall G x z S T,
-    G |-# trm_path (p_var (avar_f x)) : typ_all S T ->
-    G |-# trm_path (p_var (avar_f z)) : S ->
-    G |-# trm_app (avar_f x) (avar_f z) : T ||^ z
-| ty_new_intro_t : forall L G T ds,
-    (forall x, x \notin L ->
-      G && x ~ T ||^ x |- ds |||^ x :: T ||^ x) ->
-    G |-# trm_val (val_new T ds) : typ_bnd T
-| ty_fld_elim_t : forall G p a T,
-    G |-# trm_path p : typ_rcd { a [gen] T } ->
-    G |-# trm_path (p_sel p a) : T
-| ty_let_t : forall L G t u T U,
-    G |-# t : T ->
-    (forall x, x \notin L ->
-      G & x ~ T |- u |^ x : U) ->
-    G |-# trm_let t u : U
-| ty_rec_intro_t : forall G x T,
-    G |-# trm_path (p_var (avar_f x)) : T ||^ x ->
-    G |-# trm_path (p_var (avar_f x)) : typ_bnd T
-| ty_rec_elim_t : forall G x T,
-    G |-# trm_path (p_var (avar_f x)) : typ_bnd T ->
-    G |-# trm_path (p_var (avar_f x)) : open_typ x T
-| ty_and_intro_t : forall G x T U,
-    G |-# trm_path (p_var (avar_f x)) : T ->
-    G |-# trm_path (p_var (avar_f x)) : U ->
-    G |-# trm_path (p_var (avar_f x)) : typ_and T U
-| ty_sngl_intro_t : forall G x T,
-    G |-# trm_path (p_var (avar_f x)): T ->
-    G |-# trm_path (p_var (avar_f x)) : typ_sngl (p_var (avar_f x))
-| ty_sub_t : forall G t T U,
-    G |-# t : T ->
-    G |-# T <: U ->
-    G |-# t : U
-where "G '|-#' t ':' T" := (ty_trm_t G t T)
+    We say that [s] is well-typed with respect to [G] if
+    - [G = {(xi mapsto Ti) | i = 1, ..., n}]
+    - [s = {(xi mapsto vi) | i = 1, ..., n}]
+    - [G ⊢ vi: Ti].
 
-with ty_path_t : ctx -> path -> typ -> Prop :=
-| ty_p_intro_t: forall G x T,
-    G |-# trm_path (p_var (avar_f x)): T ->
-    G |-#\||/ p_var (avar_f x) : T
-| ty_p_rec_elim_t : forall G p T,
-    G |-#\||/ p : typ_bnd T ->
-    G |-#\||/ p : open_typ_p p T
-| ty_p_and_elim1_t : forall G p T U,
-    G |-#\||/ p: typ_and T U ->
-    G |-#\||/ p: T
-| ty_p_and_elim_2_t : forall G p T U,
-    G |-#\||/ p: typ_and T U ->
-    G |-#\||/ p: U
-| ty_p_fld_elim_t : forall G p a T,
-    G |-#\||/ p: typ_rcd {a [strong] T} ->
-    inert_sngl T ->
-    G |-#\||/ p_sel p a : T
-| ty_p_sub_t : forall G p T U,
-    G |-#\||/ p: T ->
-    G |-# T <: U ->
-    G |-#\||/ p: U
-where "G '|-#\||/' p ':' T" := (ty_path_t G p T)
+    We say that [e] is well-typed with respect to [G], denoted as [s: G]. *)
 
-with subtyp_t : ctx -> typ -> typ -> Prop :=
-| subtyp_top_t: forall G T,
-    G |-# T <: typ_top
-| subtyp_bot_t: forall G T,
-    G |-# typ_bot <: T
-| subtyp_refl_t: forall G T,
-    G |-# T <: T
-| subtyp_trans_t: forall G S T U,
-    G |-# S <: T ->
-    G |-# T <: U ->
-    G |-# S <: U
-| subtyp_and11_t: forall G T U,
-    G |-# typ_and T U <: T
-| subtyp_and12_t: forall G T U,
-    G |-# typ_and T U <: U
-| subtyp_and2_t: forall G S T U,
-    G |-# S <: T ->
-    G |-# S <: U ->
-    G |-# S <: typ_and T U
-| subtyp_fld_t: forall G a T U,
-    G |-# T <: U ->
-    G |-# typ_rcd { a [gen] T } <: typ_rcd { a [gen] U }
-| subtyp_typ_t: forall G A S1 T1 S2 T2,
-    G |-# S2 <: S1 ->
-    G |-# T1 <: T2 ->
-    G |-# typ_rcd { A >: S1 <: T1 } <: typ_rcd { A >: S2 <: T2 }
-| subtyp_sel2_t: forall G p A T,
-    G |-! trm_path p : typ_rcd { A >: T <: T } ->
-    G |-# T <: typ_path p A
-| subtyp_sel1_t: forall G p A T,
-    G |-! trm_path p : typ_rcd { A >: T <: T } ->
-    G |-# typ_path p A <: T
-| subtyp_all_t: forall L G S1 T1 S2 T2,
-    G |-# S2 <: S1 ->
-    (forall x, x \notin L ->
-       G & x ~ S2 |- T1 ||^ x <: T2 ||^ x) ->
-    G |-# typ_all S1 T1 <: typ_all S2 T2
-| subtyp_sngl_sel1_t: forall G p q A S U,
-    G |-! trm_path p: typ_sngl q ->
-    G |-# trm_path q: typ_rcd { A >: S <: U } ->
-    G |-# typ_path p A <: typ_path q A
-| subtyp_sngl_sel2_t: forall G p q A S U,
-    G |-! trm_path p: typ_sngl q ->
-    G |-# trm_path q: typ_rcd { A >: S <: U } ->
-    G |-# typ_path q A <: typ_path p A
-| subtyp_path_t: forall G a T,
-    G |-# typ_rcd { a [strong] T } <: typ_rcd { a [gen] T }
-where "G '|-#' T '<:' U" := (subtyp_t G T U).
-
-Reserved Notation "G '|-##' p ':' T" (at level 40, p at level 59).
-
-(* Invertible typing *)
-
-Inductive ty_path_inv : ctx -> path -> typ -> Prop :=
-  (* Precise typing *)
-| ty_path_i : forall G p T,
-    G |-! trm_path p : T ->
-    G |-## p : T
-| ty_sngl_i : forall G p T,
-    G |-## p: T ->
-    G |-## p : typ_sngl p
-  (* General term member subtyping *)
-| subtyp_fld_i : forall G p a T T',
-    G |-## p : typ_rcd { a [gen] T } ->
-    G |-# T <: T' ->
-    G |-## p : typ_rcd { a [gen] T' }
-  (* Strong term member subtyping *)
-| subtyp_path_i : forall G p a T,
-    G |-## p : typ_rcd { a [strong] T } ->
-    G |-## p : typ_rcd { a [gen] T }
-  (* Type member subtyping *)
-| subtyp_typ_i : forall G p A T T' U' U,
-    G |-## p : typ_rcd { A >: T <: U } ->
-    G |-# T' <: T ->
-    G |-# U <: U' ->
-    G |-## p : typ_rcd { A >: T' <: U' }
-  (* Recursive Types *)
-| ty_rec_intro_i : forall G x S,
-    G |-## (p_var (avar_f x)) : S ||^ x ->
-    G |-## (p_var (avar_f x)) : typ_bnd S
-  (* Forall *)
-| subtyp_all_i : forall L G p S T S' T',
-    G |-## p : typ_all S T ->
-    G |-# S' <: S ->
-    (forall y, y \notin L ->
-      G & y ~ S' |- T ||^ y <: T' ||^ y) ->
-    G |-## p : typ_all S' T'
-  (* And *)
-| ty_and_intro_i : forall G p S T,
-    G |-## p : S ->
-    G |-## p : T ->
-    G |-## p : typ_and S T
-  (* Tight Selection *)
-| subtyp_sel_i : forall G p q A S,
-    G |-## p : S ->
-    G |-! trm_path q : typ_rcd { A >: S <: S } ->
-    G |-## p : typ_path q A
-  (* Singleton type selection *)
-| subtyp_sngl_i: forall G p q r A,
-    G |-! trm_path p: typ_sngl r ->
-    p <> r ->
-    G |-## q: typ_path r A ->
-    G |-## q: typ_path p A
-(* Top *)
-| ty_top_i : forall G p T,
-    G |-## p : T ->
-    G |-## p : typ_top
-where "G '|-##' p ':' T" := (ty_path_inv G p T).
-
-Reserved Notation "G '|-##v' v ':' T" (at level 40, v at level 59).
-
-Inductive ty_val_inv : ctx -> val -> typ -> Prop :=
-  (* Precise typing *)
-| ty_val_i : forall G v T,
-    G |-! trm_val v : T ->
-    G |-##v v : T
-  (* Forall *)
-| subtyp_all_v : forall L G v S T S' T',
-    G |-##v v : typ_all S T ->
-    G |-# S' <: S ->
-    (forall y, y \notin L ->
-      G & y ~ S' |- T ||^ y <: T' ||^ y) ->
-    G |-##v v : typ_all S' T'
-  (* Tight Selection *)
-| subtyp_path_v : forall G v p A S,
-    G |-##v v : S ->
-    G |-! trm_path p : typ_rcd (dec_typ A S S) ->
-    G |-##v v : typ_path p A
-  (* Singleton types *)
-| subtyp_sngl_v : forall G v r A p,
-    G |-##v v: typ_path r A ->
-    G |-! trm_path p : typ_sngl r ->
-    G |-##v v: typ_path p A
-  (* Intersection introduction *)
-| ty_and_intro_v : forall G v T U,
-    G |-##v v : T ->
-    G |-##v v : U ->
-    G |-##v v : typ_and T U
-  (* Top *)
-| ty_top_v : forall G v T,
-    G |-##v v : T ->
-    G |-##v v : typ_top
-where "G '|-##v' v ':' T" := (ty_val_inv G v T).
-
-Reserved Notation "G '~~' s" (at level 40).
-
-Inductive wf_sto: ctx -> sto -> Prop :=
-| wf_sto_empty: empty ~~ empty
-| wf_sto_push: forall G s x T v,
-    G ~~ s ->
+Inductive well_typed: ctx -> sta -> Prop :=
+| well_typed_empty: well_typed empty empty
+| well_typed_push: forall G s x T v,
+    well_typed G s ->
     x # G ->
     x # s ->
-    G |- trm_val v : T ->
-    G & x ~ T ~~ s & x ~ v
-where "G '~~' s" := (wf_sto G s).
-
-(* ###################################################################### *)
-(* ###################################################################### *)
+    G ⊢ trm_val v : T ->
+    well_typed (G & x ~ T) (s & x ~ v).
 
 (** * Infrastructure *)
 
+Hint Constructors
+     inert_typ inert record_has record_dec record_typ
+     ty_trm ty_def ty_defs subtyp.
 
-(* ###################################################################### *)
-(** ** Induction principles *)
+Hint Unfold record_type.
+
+(** ** Mutual Induction Principles *)
 
 Scheme typ_mut := Induction for typ Sort Prop
-with   dec_mut := Induction for dec Sort Prop
-with   path_mut := Induction for path Sort Prop.
-Combined Scheme typ_mutind from typ_mut, dec_mut, path_mut.
+  with   dec_mut := Induction for dec Sort Prop.
+Combined Scheme typ_mutind from typ_mut, dec_mut.
 
 Scheme trm_mut  := Induction for trm  Sort Prop
-with   val_mut  := Induction for val Sort Prop
-with   def_mut  := Induction for def  Sort Prop
-with   defs_mut := Induction for defs Sort Prop.
+  with   val_mut  := Induction for val Sort Prop
+  with   def_mut  := Induction for def  Sort Prop
+  with   defs_mut := Induction for defs Sort Prop.
 Combined Scheme trm_mutind from trm_mut, val_mut, def_mut, defs_mut.
 
 Scheme ty_trm_mut    := Induction for ty_trm    Sort Prop
-with   ty_path_mut   := Induction for ty_path   Sort Prop
-with   ty_def_mut    := Induction for ty_def    Sort Prop
-with   ty_defs_mut   := Induction for ty_defs   Sort Prop.
-Combined Scheme ty_mutind from ty_trm_mut, ty_path_mut, ty_def_mut, ty_defs_mut.
+  with   ty_def_mut    := Induction for ty_def    Sort Prop
+  with   ty_defs_mut   := Induction for ty_defs   Sort Prop.
+Combined Scheme ty_mutind from ty_trm_mut, ty_def_mut, ty_defs_mut.
 
 Scheme tds_ty_trm_mut  := Induction for ty_trm    Sort Prop
-with   tds_ty_def_mut  := Induction for ty_def    Sort Prop
-with   tds_ty_defs_mut := Induction for ty_defs   Sort Prop
-with   tds_subtyp      := Induction for subtyp    Sort Prop.
+  with   tds_ty_def_mut  := Induction for ty_def    Sort Prop
+  with   tds_ty_defs_mut := Induction for ty_defs   Sort Prop
+  with   tds_subtyp      := Induction for subtyp    Sort Prop.
 Combined Scheme tds_mutind from tds_ty_trm_mut, tds_ty_def_mut, tds_ty_defs_mut, tds_subtyp.
 
 Scheme ts_ty_trm_mut  := Induction for ty_trm    Sort Prop
-with   ts_path        := Induction for ty_path   Sort Prop
-with   ts_subtyp      := Induction for subtyp    Sort Prop.
-Combined Scheme ts_mutind from ts_ty_trm_mut, ts_path, ts_subtyp.
-
-Scheme ts_ty_trm_mut_ts  := Induction for ty_trm_t    Sort Prop
-with   ts_path_ts        := Induction for ty_path_t   Sort Prop
-with   ts_subtyp_ts      := Induction for subtyp_t    Sort Prop.
-Combined Scheme ts_mutind_ts from ts_ty_trm_mut_ts, ts_path_ts, ts_subtyp_ts.
-
-Scheme ts_ty_trm_mut_t  := Induction for ty_trm_t    Sort Prop
-with   ts_path_t        := Induction for ty_path_t   Sort Prop.
-Combined Scheme ts_mutind_t from ts_ty_trm_mut_t, ts_path_t.
+  with   ts_subtyp      := Induction for subtyp    Sort Prop.
+Combined Scheme ts_mutind from ts_ty_trm_mut, ts_subtyp.
 
 Scheme rules_trm_mut    := Induction for ty_trm    Sort Prop
-with   rules_path_mut   := Induction for ty_path   Sort Prop
-with   rules_def_mut    := Induction for ty_def    Sort Prop
-with   rules_defs_mut   := Induction for ty_defs   Sort Prop
-with   rules_subtyp     := Induction for subtyp    Sort Prop.
-Combined Scheme rules_mutind from rules_trm_mut, rules_path_mut, rules_def_mut, rules_defs_mut, rules_subtyp.
+  with   rules_def_mut    := Induction for ty_def    Sort Prop
+  with   rules_defs_mut   := Induction for ty_defs   Sort Prop
+  with   rules_subtyp     := Induction for subtyp    Sort Prop.
+Combined Scheme rules_mutind from rules_trm_mut, rules_def_mut, rules_defs_mut, rules_subtyp.
 
-(* ###################################################################### *)
-(** ** Tactics *)
+Scheme rcd_dec_mut := Induction for record_dec Sort Prop
+  with rcd_typ_mut := Induction for record_typ Sort Prop
+  with inert_mut   := Induction for inert_typ Sort Prop.
+Combined Scheme rcd_mutind from rcd_dec_mut, rcd_typ_mut, inert_mut.
+
+(** * Tactics *)
+
+(** Tactics for generating fresh variables. *)
 
 Ltac gather_vars :=
   let A := gather_vars_with (fun x : vars      => x         ) in
   let B := gather_vars_with (fun x : var       => \{ x }    ) in
   let C := gather_vars_with (fun x : ctx       => (dom x) \u (fv_ctx_types x)) in
-  let D := gather_vars_with (fun x : sto       => dom x     ) in
+  let D := gather_vars_with (fun x : sta        => dom x \u fv_sta_vals x) in
   let E := gather_vars_with (fun x : avar      => fv_avar  x) in
   let F := gather_vars_with (fun x : trm       => fv_trm   x) in
   let G := gather_vars_with (fun x : val       => fv_val   x) in
   let H := gather_vars_with (fun x : def       => fv_def   x) in
   let I := gather_vars_with (fun x : defs      => fv_defs  x) in
   let J := gather_vars_with (fun x : typ       => fv_typ   x) in
-  let K := gather_vars_with (fun x : path      => fv_path  x) in
-  constr:(A \u B \u C \u D \u E \u F \u G \u H \u I \u J \u K).
+  constr:(A \u B \u C \u D \u E \u F \u G \u H \u I \u J).
 
 Ltac pick_fresh x :=
   let L := gather_vars in (pick_fresh_gen L x).
 
-(*Ltac in_empty_contradiction :=
-  solve [match goal with
-  | H: _ \in \{} |- _ => rewrite in_empty in H; exfalso; exact H
-end].
-
-Ltac eq_specialize :=
-  repeat match goal with
-  | H:                 _ = _ -> _ |- _ => specialize (H         eq_refl)
-  | H: forall _      , _ = _ -> _ |- _ => specialize (H _       eq_refl)
-  | H: forall _ _    , _ = _ -> _ |- _ => specialize (H _ _     eq_refl)
-  | H: forall _ _ _  , _ = _ -> _ |- _ => specialize (H _ _ _   eq_refl)
-  | H: forall _ _ _ _, _ = _ -> _ |- _ => specialize (H _ _ _ _ eq_refl)
-  end.
-
-Ltac crush := eq_specialize; eauto.*)
-
 Tactic Notation "apply_fresh" constr(T) "as" ident(x) :=
   apply_fresh_base T gather_vars x.
 
-Hint Constructors
-     ty_trm ty_def ty_defs subtyp ty_trm_t subtyp_t ty_trm_p
-     ty_path ty_path_t
-     ty_path_inv ty_val_inv inert_sngl inert_typ inert
-     wf_sto record_has.
+Ltac fresh_constructor :=
+  apply_fresh ty_new_intro as z ||
+  apply_fresh ty_all_intro as z ||
+  apply_fresh ty_let as z ||
+  apply_fresh subtyp_all as z; auto.
 
-Lemma fresh_push_eq_inv: forall A x a (E: env A),
-  x # (E & x ~ a) -> False.
-Proof.
-  intros. rewrite dom_push in H. false H. rewrite in_union.
-  left. rewrite in_singleton. reflexivity.
-Qed.
+(** Tactics for naming cases in case analysis. *)
+
+Open Scope string_scope.
+
+Ltac move_to_top x :=
+  match reverse goal with
+  | H : _ |- _ => try move x after H
+  end.
+
+Tactic Notation "assert_eq" ident(x) constr(v) :=
+  let H := fresh in
+  assert (x = v) as H by reflexivity;
+  clear H.
+
+Tactic Notation "Case_aux" ident(x) constr(name) :=
+  first [
+    set (x := name); move_to_top x
+  | assert_eq x name; move_to_top x
+  | fail 1 "because we are working on a different case" ].
+
+Tactic Notation "Case" constr(name) := Case_aux Case name.
+Tactic Notation "SCase" constr(name) := Case_aux SCase name.
+Tactic Notation "SSCase" constr(name) := Case_aux SSCase name.
+Tactic Notation "SSSCase" constr(name) := Case_aux SSSCase name.
+Tactic Notation "SSSSCase" constr(name) := Case_aux SSSSCase name.
+Tactic Notation "SSSSSCase" constr(name) := Case_aux SSSSSCase name.
+
+(** Automatically destruct premises *)
+Ltac destruct_all :=
+  repeat match goal with
+  | [ H : exists x, _ |- _ ]  => destruct H
+  | [ H : ?A /\ ?B |- _ ] => destruct H
+  | [ H : ?A \/ ?B |- _ ] => destruct H
+  end.
+
+Ltac omega := Coq.omega.Omega.omega.
