src/extensions/paths/README.md
@@ -1,5 +1,0 @@
-# DOT with Extended Paths
-
-We are working on an extension for DOT that supports type selection on paths of arbitrary length, as opposed to type selection on variables. For example, we allow a type of the form `x.a.b.A` instead of only `x.A`.
-
-This is work in progress. The definition of the type system can be found in `Definitions.v`.
